fix of the temporal transition in progress

theories/Environment/Resources.v
@@ -24,6 +24,13 @@ Import St.
 Definition multi_shift (lbs : list lvl) (ks : list lvl) (t : t) :=
   List.fold_right (fun lbk acc => shift (fst lbk) (snd lbk) acc) t (List.combine lbs ks).
 
+(** **** New key *)
+
+Definition max_key (t : t) := fold (Nat.max) t 0.
+
+Definition new_key (t : t) := 
+  if is_empty t then 0 else S (max_key t).
+
 (** *** Property *)
 
 (** **** [multi_shift] property *)
@@ -33,6 +40,148 @@ Proof.
   intros lbs' lbs Heqlbs ks' ks Heqks r1 r2 Heqr; subst.
   unfold eq in Heqr; apply eq_leibniz in Heqr. 
   now rewrite Heqr.
+Qed.
+
+(** **** [max_key] property *)
+
+#[export] Instance max_key_eq : Proper (eq ==> Logic.eq) max_key.
+Proof.
+  intros x y Heq.
+  apply eq_leibniz in Heq; now subst.
+Qed.
+
+Lemma max_key_Empty_spec (m : t) : Empty m -> max_key m = 0.
+Proof. 
+  intro HEmp; unfold max_key.
+  rewrite fold_1; auto.
+  constructor; auto.
+  intros x y z Heq Heq'; now subst.
+Qed.
+
+Lemma max_key_empty_spec : max_key empty = 0.
+Proof.
+  unfold max_key; now rewrite fold_empty.
+Qed.
+
+Lemma max_key_Add_spec (m m' : t) x :
+  ~ In x m -> Add x m m' ->
+  (max_key m' = x /\ max_key m <= x) \/ (max_key m' = max_key m /\ max_key m > x).
+Proof.
+  intros HnIn HAdd; unfold max_key.
+  apply Add_inv in HAdd; subst.
+  rewrite fold_add; eauto; try lia.
+  - constructor; auto.
+    intros w y z H H1; now subst.
+  - intros n' n Heqn p' p Heqp; now subst.
+  - intros n p q; lia.
+Qed.
+
+Lemma max_key_Add_ge_spec (m m' : t) x :
+  ~ In x m -> Add x m m' ->  max_key m <= x -> max_key m' = x.
+Proof.
+  intros HnIn HAdd Hmax.
+  apply max_key_Add_spec in HAdd; auto.
+  destruct HAdd as [[Heq Hle] | [Heq Hgt]]; auto.
+  lia.
+Qed.
+
+Lemma max_key_Add_lt_spec (m m' : t) x :
+  ~ In x m -> Add x m m' ->  max_key m > x -> max_key m' = max_key m.
+Proof.
+  intros HnIn HAdd Hmax.
+  apply max_key_Add_spec in HAdd; auto.
+  destruct HAdd as [[Heq Hle] | [Heq Hgt]]; auto.
+  lia.
+Qed.
+
+Lemma max_key_add_spec (m : t) x :
+  ~ In x m -> (max_key (add x m) = x /\ max_key m <= x) \/ 
+              (max_key (add x m) = max_key m /\ max_key m > x).
+Proof.
+  intro HnIn.
+  eapply max_key_Add_spec; auto.
+Qed.
+
+Lemma max_key_add_ge_spec (m : t) x :
+  ~ In x m -> max_key m <= x -> max_key (add x m) = x.
+Proof.
+  intro HnIn.
+  eapply max_key_Add_ge_spec; auto.
+Qed.
+
+Lemma max_key_add_lt_spec (m : t) x :
+  ~ In x m -> max_key m > x -> max_key (add x m) = max_key m.
+Proof.
+  intro HnIn.
+  eapply max_key_Add_lt_spec; auto.
+Qed.
+
+Lemma max_key_add_spec_1 (m m' : t) x :
+  ~ In x m -> ~ In x m' ->
+  max_key m = max_key m' -> max_key (add x m) = max_key (add x m').
+Proof.
+  intros HnIn HnIn'. 
+  apply max_key_add_spec in HnIn as HI. 
+  apply max_key_add_spec in HnIn' as HI'.
+  destruct HI as [[Heq1 Hleb1] | [Heq1 Hgt1]];
+  destruct HI' as [[Heq2 Hleb2] | [Heq2 Hgt2]]; subst; try lia.
+Qed.
+
+(** **** [new_key] property *)
+
+Lemma new_key_empty_spec : new_key empty = 0.
+Proof. now unfold new_key; simpl. Qed.
+
+#[export] Instance new_key_eq : Proper (eq ==> Logic.eq) new_key.
+Proof. 
+  intros s1 s2 Heq.
+  apply eq_leibniz in Heq; now subst.
+Qed.
+
+Lemma new_key_add_spec (x: lvl) (t : t) :
+  ~In x t -> (new_key (add x t) = S x /\ new_key t <= S x) \/ 
+               (new_key (add x t) = new_key t /\ new_key t > S x).
+Proof.
+  intro HnIn.
+  unfold new_key.
+  assert (is_empty (add x t) = false).
+  - apply Bool.not_true_is_false.
+    intro Hc.
+    rewrite is_empty_spec in Hc.
+    apply (Hc x).
+    apply add_spec; auto.
+  - rewrite H.
+    apply max_key_add_spec in HnIn as [[Heq Hle] | [Heq Hgt]].
+    -- left; split; auto.
+       destruct (is_empty t); lia.
+    -- rewrite Heq.
+       destruct (is_empty t) eqn:Hemp.
+       + rewrite max_key_Empty_spec in Hgt; try lia.
+         now rewrite <- is_empty_spec.
+       + right; split; auto; lia.
+Qed.
+
+Lemma new_key_add_lt_spec (x: lvl) (t : t) :
+  ~ In x t -> new_key t > S x -> new_key (add x t) = new_key t.
+Proof.
+  intros HnIn Hgt.
+  apply new_key_add_spec in HnIn as [[Heq Hlt] | [Heq Hgt']]; auto.
+  lia.
+Qed. 
+
+Lemma new_key_add_ge_spec (x: lvl) (t : t) :
+  ~ In x t -> new_key t <= S x -> new_key (add x t) = S x.
+Proof.
+  intros HnIn Hgt.
+  apply new_key_add_spec in HnIn as [[Heq Hlt] | [Heq Hgt']]; auto.
+  lia.
+Qed.
+
+Lemma new_key_max_spec (x: lvl) (t : t) :
+  ~ In x t -> new_key (add x t) = max (new_key t) (S x).
+Proof.
+  intro HnIn.
+  apply new_key_add_spec in HnIn as [[Heq Hlt] | [Heq Hgt']]; lia.
 Qed.
 
 (** **** [valid] Wormholes specification *)
@@ -92,6 +241,7 @@ Delimit Scope resources_scope with rs.
 Definition resources := Resources.t.
 
 Infix "⊩" := Resources.valid (at level 20, no associativity) : resources_scope. 
+Notation "t '⁺'" := (Resources.new_key t) (at level 16) : resources_scope.
 Notation "'[⧐' lb '–' k ']' t" := (Resources.shift lb k t) (at level 65, right associativity) : resources_scope.
 Notation "'[⧐⧐' lb '–' k ']' t" := (Resources.multi_shift lb k t) (at level 65, right associativity) : resources_scope.
 
@@ -103,5 +253,6 @@ Import Resources.
 #[export] Instance resources_valid_proper :  Proper (Level.eq ==> eq ==> iff) valid := _.
 #[export] Instance resources_shift_proper : Proper (Level.eq ==> Level.eq ==> eq ==> eq) shift := shift_eq.
 #[export] Instance resources_multi_shift_proper : Proper (Logic.eq ==> Logic.eq ==> eq ==> Logic.eq) multi_shift := _.
+#[export] Instance resources_new_key_proper : Proper (eq ==> Logic.eq) new_key := _.
 
 End ResourcesNotations.
