theories/Environment/Stock.v
@@ -1,13 +1,13 @@
 From Coq Require Import Lia.
-From Mecha Require Import Resource Resources Term REnvironment Cell ReaderStock.
+From Mecha Require Import Resource Resources Term REnvironment Cell SREnvironment.
 From DeBrLevel Require Import LevelInterface PairLevel.
 From MMaps Require Import MMaps.
 Import ResourceNotations TermNotations CellNotations REnvironmentNotations
-       ReaderStockNotations ResourcesNotations SetNotations.
+       SREnvironmentNotations ResourcesNotations SetNotations.
 
 (** * Environment - Virtual Resource Environment
 
-  In the functional transition there are two kind of environment: the resource environment and the stock. The former, defined in [REnvironment.v], represents the local memory during an instant. The latter, defined here, keeps local resource names with their initial value. This environment is a pair split into a map, defined in [ReaderStock.v], which maps local resource names, used for a reading interaction, to terms, and a set which keeps 'writing' local resource names.   
+  In the functional transition there are two kind of environment: the resource environment and the stock. The former, defined in [REnvironment.v], represents the local memory during an instant. The latter, defined here, keeps local resource names with their initial value. This environment is a pair split into a map, defined in [SREnvironment.v], which maps local resource names, used for a reading interaction, to terms, and a set which keeps 'writing' local resource names.   
 *)
 
 (** ** Module - Virtual Resource Environment *)
@@ -15,61 +15,70 @@ Module Stock <: IsLvlET.
 
 (** *** Definition *)
 
-Include IsLvlPairET ReaderStock Resources.
+Include IsLvlPairET SREnvironment Resources.
 Module RE := REnvironment.
-Module REA := ReaderStock.
+Module SRE := SREnvironment.
 Module RS := Resources.St.
 
 Open Scope resources_scope.
 Open Scope set_scope.
 
 (** **** Projections *)
-Definition readers (W : t) : 𝐖ᵣ := fst W.
+Definition readers (W : t) : 𝐄 := fst W.
 Definition writers (W : t) : resources := snd W.
 
 (** **** Empty stock 
 
   A stock is empty if and only if both components are empty.
 *)
-Definition empty : t := (∅%rk,∅). 
+Definition empty : t := (∅%sr,∅). 
 
 (** **** Initialize the resource environment
 
   For each instant, the resource environment has to be initialize for its global resource names and its local ones. The latter is done by picking information in the stock. We define [init_locals] which takes a stock [W] and a resource environment [V] and produces a new resource environment with all elements of [V] and readers and writers, stored in [W], initialized.
 *)
 Definition init_locals (W : t) (V : 𝐕) : 𝐕 :=
-  REA.init_readers (readers W) (RE.init_writers (writers W)  V).
+  SRE.init_readers (readers W) (RE.init_writers (writers W)  V).
+
+(** **** Update the resource environment 
+
+  For each instant, the resource environment is updated at the end. Each local resources may have a new initial term for the next instant. We defined [update_locals] which takes a stock [W] and a resource environment [V] and produces a new stock.
+*)
+Definition update_locals (W : t) (V : 𝐕) : t := (SRE.update_readers (readers W) V, writers W).
 
 (** **** Add
 
   In the stock, we add a three elements: the reader resource name [rr], the writer resource name [rw] and the initial value [v]. [rr] and [v] are added in the first member of the pair, which is a map from [ReaderStock.v], and the last elements is added in the set of writers, i.e. in the second member of the pair.
 *)
 Definition add (rr rw : resource) (v : Λ) (W : t) : t :=
-  (⌈ rr ⤆ v ⌉ (readers W),rw +: (writers W))%rk.
+  (⌈ rr ⤆ v ⌉ (readers W),rw +: (writers W))%sr.
 
 (** **** Union
 
   The union between two stocks is the point-to-point union between each component.
 *)
-Definition union (W W' : t) := ((readers W ∪ readers W')%rk, writers W ∪ writers W').
+Definition union (W W' : t) := ((readers W ∪ readers W')%sr, writers W ∪ writers W').
 
 (** **** In
 
   A resource name is in the stock if it is, at least, in one member of the stock.
 *)
-Definition In (r : resource) (W : t) := (r ∈ readers W)%rk \/ (r ∈ writers W).
+Definition In (r : resource) (W : t) := (r ∈ readers W)%sr \/ (r ∈ writers W).
 
 (** **** Find
 
   A data can be find only in the first member of the stock.
 *)
-Definition find (r : resource) (W : t) := (readers W) ⌊r⌋%rk.
+Definition find (r : resource) (W : t) := (readers W) ⌊r⌋%sr.
 
 (** **** Halts
 
   In the functional transition proofs, we assume that all elements in the input resource environment halts. The resource environment depends on the stock for its initialization in the temporal transition. Consequently, we also need to define the halts property on the stock.
 *)
-Definition halts (k : lvl) (W : t) := REA.halts k (readers W).
+Definition halts (k : lvl) (W : t) := SRE.halts k (readers W).
+
+(** **** New key *)
+Definition new_key (W : t) := max ((readers W)⁺)%sr ((writers W)⁺)%s.
 
 (** *** Property *)
 
@@ -80,10 +89,10 @@ Lemma init_locals_in_iff (r : resource) (W : t) (V : 𝐕) :
 Proof.
   split; unfold init_locals, In; destruct W as [rW wW]; simpl.
   - intro HIn. 
-    apply REA.init_readers_in_iff in HIn as [| HIn]; auto.
+    apply SRE.init_readers_in_iff in HIn as [| HIn]; auto.
     apply RE.init_writers_in_iff in HIn as [|]; auto.
   - intro HIns. 
-    apply REA.init_readers_in_iff.
+    apply SRE.init_readers_in_iff.
     rewrite RE.init_writers_in_iff.
     destruct HIns as [[HIn | HIn] | HIn]; auto.
 Qed.
@@ -92,8 +101,66 @@ Lemma init_locals_find_spec (r : resource) (v : 𝑣) (W : t) (V : 𝐕) :
  (init_locals W V)⌊r⌋%re = Some v -> In r W \/ V⌊r⌋%re = Some v.
 Proof.
   unfold init_locals, In; destruct W as [rW wW]; simpl; intro Hfi. 
-  apply REA.init_readers_find_spec in Hfi as [| Hfi]; auto.
+  apply SRE.init_readers_find_spec in Hfi as [| Hfi]; auto.
   apply RE.init_writers_find_spec in Hfi as [|]; auto.
+Qed.
+
+Lemma init_locals_find_spec_1 (r : resource) (v : 𝑣) (W : t) (V : 𝐕) :
+ (init_locals W V)⌊r⌋%re = Some v -> 
+ (readers W)⌊r⌋%sr = Some (Cell.extract v) \/ 
+ (RE.init_writers (writers W) V)⌊r⌋%re = Some v.
+Proof.
+  unfold init_locals, In; destruct W as [rW wW]; simpl; intro Hfi. 
+  apply SRE.init_readers_find_spec_1 in Hfi as [| Hfi]; auto; right.
+Qed.
+
+Lemma init_locals_find_inp_spec (rs : t) (V : 𝐕) (r : resource) (v : 𝑣) :
+  (forall r, V⌊r⌋%re = Some v -> exists v', Logic.eq v (Cell.inp v')) ->
+  ((init_locals rs V)⌊r⌋)%re = Some v -> exists v', Logic.eq v (Cell.inp v'). 
+Proof.
+  unfold init_locals; intros Ht Hfi.
+  apply SRE.init_readers_find_inp_spec in Hfi; auto.
+  intros r' HfV.
+  apply RE.init_writers_find_inp_spec in HfV; auto.
+Qed.
+
+Lemma init_locals_in_unused (W : t) (V : 𝐕) (r : resource) :
+  In r W -> RE.unused r (init_locals W V).
+Proof.
+  intro HIn; unfold In, init_locals in *; destruct W as [Rw Ww].
+  destruct HIn as [HIn | HIn]; simpl in *.
+  - now apply SRE.init_readers_in_unused.
+  - apply SRE.init_readers_unused. 
+    now apply RE.init_writers_in_unused.
+Qed.
+
+
+Lemma init_locals_unused (r : resource) (W : t) (V : 𝐕) :
+  RE.unused r V -> RE.unused r (Stock.init_locals W V).
+Proof.
+  unfold Stock.init_locals; intro Hunsd.
+  apply SRE.init_readers_unused.
+  now apply RE.init_writers_unused.
+Qed.
+
+Lemma init_locals_new_key (V : 𝐕) (t : t) : ((init_locals t V)⁺)%re = max (new_key t) (V⁺)%re.
+Proof.
+  destruct t; unfold init_locals, new_key; simpl.
+  rewrite SRE.init_readers_new_key.
+  rewrite RE.init_writers_new_key.
+  lia.
+Qed.
+
+(** **** [update_locals] property *)
+
+Lemma update_locals_in_iff (r : resource) (W : t) (V : 𝐕) :
+  In r (update_locals W V) <-> In r W.
+Proof.
+  split; unfold init_locals, In; destruct W as [rW wW]; simpl.
+  - intros [HIn |]; auto. 
+    apply SRE.update_readers_in_iff in HIn; auto.
+  - intros [HIn |]; auto; left. 
+    now apply SRE.update_readers_in_iff.
 Qed.
     
 (** **** [In] property  *)
@@ -101,7 +168,7 @@ Qed.
 Lemma empty_in_spec (r : resource) : ~ In r empty.
 Proof.
   unfold In, empty; simpl; intros [HIn | HIn].
-  - revert HIn; apply REA.not_in_empty.
+  - revert HIn; apply SRE.not_in_empty.
   - inversion HIn.
 Qed.
 
@@ -111,9 +178,9 @@ Proof.
   unfold add, In; destruct W as [rw wW]; simpl; split.
   - intros [HIn | HIn].
     -- destruct (Resource.eq_dec k r) as [| Hneq]; subst; auto. 
-       rewrite REA.add_neq_in_iff in HIn; auto.
+       rewrite SRE.add_neq_in_iff in HIn; auto.
     -- apply RS.add_spec in HIn as [|]; auto.
-  - rewrite REA.add_in_iff; rewrite RS.add_spec.
+  - rewrite SRE.add_in_iff; rewrite RS.add_spec.
     intros [Heq | [Heq | [HIn | HIn]]]; subst; auto.
 Qed.
 
@@ -121,7 +188,7 @@ Lemma union_spec (r : resource) (W W' : t) :
   In r (union W W') <-> In r W \/ In r W'.
 Proof.
   unfold In,union; destruct W,W'; simpl.
-  rewrite REA.extend_in_iff; rewrite RS.union_spec.
+  rewrite SRE.extend_in_iff; rewrite RS.union_spec.
   split; intros [[|] | [|]]; auto.
 Qed.
 
@@ -132,9 +199,9 @@ Lemma union_find_spec (r : resource) (v : Λ) (W W' : t) :
   find r (union W W') = Some v -> find r W = Some v \/ find r W' = Some v.
 Proof.
   unfold find, union; destruct W,W'; simpl; intro HM.
-  apply REA.find_2 in HM. 
-  apply REA.extend_mapsto_iff in HM as [HM | [HM _]];
-  apply REA.find_1 in HM; auto.
+  apply SRE.find_2 in HM. 
+  apply SRE.extend_mapsto_iff in HM as [HM | [HM _]];
+  apply SRE.find_1 in HM; auto.
 Qed.
 
 (** **** [valid] poperty *)
@@ -142,7 +209,7 @@ Qed.
 Lemma valid_empty_spec (k : lvl) : valid k empty.
 Proof.
   unfold valid, empty; simpl; split.
-  - apply REA.valid_empty_spec.
+  - apply SRE.valid_empty_spec.
   - apply Resources.valid_empty_spec.
 Qed.
 
@@ -151,7 +218,7 @@ Lemma valid_add_spec (k : lvl) (r r' : resource) (v : Λ) (W : t) :
 Proof.
   unfold valid; destruct W as [rW wW]; simpl. 
   intros Hvr Hvr' Hvv [HvrW HvwW]; split.
-  - apply REA.valid_add_spec; auto.
+  - apply SRE.valid_add_spec; auto.
   - apply Resources.valid_unfold; intros r1 HIn.
     apply RS.add_spec in HIn as [|]; subst; auto.
 Qed.
@@ -161,7 +228,7 @@ Lemma valid_union_spec (k : lvl) (W W' : t) :
 Proof.
   unfold valid; destruct W,W'; simpl. 
   intros [[HvrW HvwW] [HvrW' HvwW']]; split.
-  - apply REA.valid_extend_spec; auto.
+  - apply SRE.valid_extend_spec; auto.
   - apply Resources.valid_union_iff; split; auto.
 Qed.
 
@@ -170,7 +237,7 @@ Lemma valid_in_spec (k : lvl) (r : resource) (W : t) :
 Proof.
   unfold In, valid; destruct W as [rW wW]; simpl.
   intros [HIn | HIn] [HvrW HvwW].
-  - eapply REA.valid_in_spec in HIn; eauto.
+  - eapply SRE.valid_in_spec in HIn; eauto.
   - eapply Resources.valid_in_spec; eauto.
 Qed.
 
@@ -179,13 +246,28 @@ Lemma valid_in_iff (m n k : lvl) (W : t) :
 Proof.
   unfold valid, shift, In; destruct W as [rW wW]; simpl.
   intros [Hvr Hvw]; split; intros [HIn | HIn].
-  - now left; rewrite ReaderStock.valid_in_iff in HIn.
+  - now left; rewrite SRE.valid_in_iff in HIn.
   - now right; rewrite Resources.valid_in_iff in HIn.
-  - now left; rewrite ReaderStock.valid_in_iff.
+  - now left; rewrite SRE.valid_in_iff.
   - now right; rewrite Resources.valid_in_iff.
 Qed.
 
+Lemma init_locals_valid (k : lvl) (V : 𝐕) (t : t) :
+  valid k t -> (k ⊩ V)%re -> (k ⊩ init_locals t V)%re.
+Proof.
+Admitted.
 
+(** **** [new_key] property *)
+
+Lemma new_key_empty_spec : new_key empty = 0.
+Proof.
+  unfold new_key, empty.
+  simpl (readers (∅, ∅%s) ⁺)%sr.
+  simpl (writers (∅%sr, ∅) ⁺).
+  rewrite SRE.Ext.new_key_empty_spec. 
+  rewrite Resources.new_key_empty_spec.
+  now simpl. 
+Qed.
 (** **** [shift] property *)
 
 Lemma shift_in_iff (m n : lvl) (r : resource) (W : t) :
@@ -193,9 +275,9 @@ Lemma shift_in_iff (m n : lvl) (r : resource) (W : t) :
 Proof.
   unfold In, shift; destruct W as [rW wW]; simpl; 
   split; intros [HIn | HIn].
-  - left. now apply REA.shift_in_iff.
+  - left. now apply SRE.shift_in_iff.
   - right; now apply Resources.shift_in_iff.
-  - left. rewrite REA.shift_in_iff; eauto.
+  - left. rewrite SRE.shift_in_iff; eauto.
   - right; rewrite Resources.shift_in_iff; eauto.
 Qed.
 
@@ -203,7 +285,7 @@ Lemma shift_in_e_spec (m n : lvl) (r : resource) (W : t) :
   In r (shift m n W) -> exists r', (r =  ([⧐ m – n] r')%r)%type.
 Proof.
   unfold In,shift; destruct W as [rW wW]; simpl; intros [HIn | HIn].
-  - apply REA.shift_in_e_spec in HIn; auto.
+  - apply SRE.shift_in_e_spec in HIn; auto.
   - apply Resources.shift_in_e_spec in HIn as [r' [Heq _]]; subst.
     now exists r'.
 Qed.
@@ -223,37 +305,38 @@ Lemma halts_init_locals (k : lvl) (W : t) (V : 𝐕) :
 Proof.
   unfold halts, init_locals; destruct W as [rW wW]; simpl.
   intros HvrW HvV.
-  apply REA.halts_init_readers; auto.
+  apply SRE.halts_init_readers; auto.
   now apply RE.halts_init_writers.
 Qed.
 
-(* Lemma halts_update (k : lvl) (W : t) (V : 𝐕) :
-  RE.halts k V -> halts k W -> halts k (update W V).
+Lemma halts_update_locals (k : lvl) (W : t) (V : 𝐕) :
+  RE.halts k V -> halts k W -> halts k (update_locals W V).
 Proof.
-  intros. unfold halts,update; simpl; destruct W; simpl.
-  apply REA.halts_env_from_renv; auto.
-Qed. *)
+  intros HltV HltW; unfold halts,update_locals.
+  destruct W as [Rw Ww]; simpl.
+  apply SRE.halts_update_readers; auto.
+Qed.
 
 Lemma halts_weakening (m n : lvl) (W : t) : 
   m <= n -> halts m W -> halts n (shift m (n - m) W).
 Proof.
   unfold halts, shift; destruct W as [rW wW]. 
   simpl; intros Hle HvrW.
-  now apply REA.halts_weakening.
+  now apply SRE.halts_weakening.
 Qed.
 
 Lemma halts_union_spec (k : lvl) (W W' : t) :
   halts k W /\ halts k W' -> halts k (union W W').
 Proof.
   unfold halts; destruct W,W'; simpl; intro Hlt. 
-  now apply REA.halts_union_spec.
+  now apply SRE.halts_union_spec.
 Qed.
 
 Lemma halts_add_spec (k : lvl) (r r' : resource) (v : Λ) (W : t) :
   (Evaluation_Transition.halts k v) /\ halts k W -> halts k (add r r' v W).
 Proof.
   unfold halts, add; destruct W as [rW wW]; simpl; intro Hv.
-  now apply REA.halts_add_spec.
+  now apply SRE.halts_add_spec.
 Qed.
 
 
@@ -286,6 +369,15 @@ Proof.
   - now rewrite HeqW.
 Qed. 
 
+#[export] Instance new_key_eq : Proper (eq ==> Logic.eq) new_key.
+Proof.
+  intros [rt1 wt1] [rt2 wt2] Heq.
+  repeat red in Heq; unfold RelationPairs.RelCompFun in Heq; simpl in *.
+  destruct Heq as [Heqr Heqw].
+  unfold new_key; simpl.
+  now rewrite Heqr, Heqw.
+Qed.
+
 End Stock.
 
 (** ---- *)
@@ -302,10 +394,11 @@ Delimit Scope stock_scope with sk.
 Definition 𝐖 := Stock.t.
 
 Infix "∈" := Stock.In (at level 60, no associativity) : stock_scope. 
-Notation "r '∉' Re" := (~ (Stock.In r Re)) (at level 75, no associativity) : stock_scope. 
+Notation "r '∉' t" := (~ (Stock.In r t)) (at level 75, no associativity) : stock_scope. 
+Notation "t '⁺'" := (Stock.new_key t) (at level 16) : stock_scope.
 Notation "∅" := Stock.empty (at level 0, no associativity) : stock_scope. 
-Notation "R '⌊' x '⌋'"  := (Stock.find x R) (at level 15, x constr) : stock_scope.
-Notation "⌈ x '~' x1 ⤆ v '⌉' R"  := (Stock.add x x1 v R) 
+Notation "t '⌊' x '⌋'"  := (Stock.find x t) (at level 15, x constr) : stock_scope.
+Notation "⌈ x '~' x1 ⤆ v '⌉' t"  := (Stock.add x x1 v t) 
                                      (at level 15, x constr, v constr) : stock_scope.
 Notation "'[⧐' lb '–' k ']' t" := (Stock.shift lb k t) 
                                    (at level 65, right associativity) : stock_scope.
@@ -324,5 +417,6 @@ Import Stock.
 #[export] Instance in_stk : Proper (Logic.eq ==> eq ==> iff) In := _.
 #[export] Instance find_stk : Proper (Logic.eq ==> eq ==> Logic.eq) find := _.
 #[export] Instance add_stk : Proper (Resource.eq ==> Resource.eq ==> Term.eq ==> eq ==> eq) add := _.
+#[export] Instance new_key_stk : Proper (eq ==> Logic.eq) new_key := _.
 
 End StockNotations.
