theories/Environment/Inputs.v
@@ -1,0 +1,30 @@
+From Coq Require Import Lia Arith.PeanoNat Classical_Prop Morphisms SetoidList.
+From Mecha Require Import Resource Resources Term Cell REnvironment.
+From Mecha Require Evaluation_Transition.
+From DeBrLevel Require Import LevelInterface MapLevelInterface MapLevel MapExtInterface MapExt.
+Import ResourceNotations TermNotations CellNotations
+       ResourcesNotations SetNotations REnvironmentNotations.
+
+(** * Environments - Inputs *)
+
+(** ** Module - Inputs *)
+
+Module Inputs <: IsLvlET.
+
+(** *** Definition *)
+
+Include MapLvlD.MakeLvlMapLVLD Term.
+Import Raw Ext.
+
+Module RE := REnvironment.
+Open Scope renvironment_scope.
+
+(** **** Initialize the resource environment *)
+
+Definition init_globals_func (r : resource) (v : Λ) (V : 𝐕) := ⌈r ⤆ ⩽ v … ⩾⌉ V.
+
+Definition init_globals (t : t) : 𝐕 := fold init_globals_func t ∅.
+
+
+
+End Inputs.
