theories/Environment/SREnvironment.v
@@ -1,0 +1,795 @@
+From Coq Require Import Lia Arith.PeanoNat Morphisms.
+From Mecha Require Import Resource Resources Term REnvironment Cell.
+From DeBrLevel Require Import LevelInterface MapLevelInterface MapLevel MapExtInterface MapExt.
+Import ResourceNotations TermNotations REnvironmentNotations CellNotations
+       ResourcesNotations SetNotations.
+
+
+(** * Environment - Simple Resource Environment
+
+  In the functional transition there are two kind of environment: the resource environment and the stock. The former, defined in [REnvironment.v], represents the local memory during an instant. The latter, defined in [Stock.v], keeps local resource names with their initial value. In addition, in the temporal transition we also need a simple map between resource names and terms.
+*)
+
+(** ** Module - Virtual Resource Environment - Reader *)
+Module SREnvironment <: IsLvlET.
+
+Include MapLvlD.MakeLvlMapLVLD Term.
+Import Raw Ext.
+
+Module ET := Evaluation_Transition.
+Module RE := REnvironment.
+
+(** *** Definition *)
+
+(** **** Initialize an environment
+
+  For each instant, local resource names that represent a reading interaction have their memory cells initialized as unused with a certain term. Same idea for global input resource names in the temporal transition. This function takes a reader environment [rs] and an environement [V] and produces an environment where all resource names in [rs] are initialized.
+*)
+Definition init_func (r : resource) (v : Λ) (V : 𝐕) := (⌈ r ⤆ ⩽ v … ⩾ ⌉ V)%re.
+
+Definition init_readers (t : t) (V : 𝐕) := fold init_func t V.
+Definition init_globals (t : t) : 𝐕 := init_readers t (∅)%re.
+
+
+(** **** Update the resource environment 
+
+  For each instant, the resource environment is updated at the end. Each local resources may have a new initial term for the next instant. We defined [update_readers] which takes a stock [W] and a resource environment [V] and produces a new stock.
+*)
+Definition update_readers_func (V : 𝐕) (r : resource) (v : Λ) (rs : t) : t :=
+  match (V⌊r⌋)%re with 
+    | Some (⩽ … v' ⩾) =>  add r v' rs
+    |  _ => add r v rs
+  end.
+
+Definition update_readers (rs : t) (V : 𝐕) : t := fold (update_readers_func V) rs empty.
+
+(** **** Halts 
+
+  In the functional transition proofs, we assume that all elements in the virtual resource environment [W] halts. Thus, we define this property here with [For_all].
+  An environment has the halting property if and only if each term in it halts. 
+*)
+Definition halts (k : lvl) := For_all (fun _ d => ET.halts k d).
+
+(** *** Property *)
+
+(** **** [extend] property *)
+ 
+Lemma extend_Empty_left_spec (rs rs' : t) :
+  Empty rs -> eq (extend rs rs') rs'.
+Proof.
+  intro HEmp; unfold extend.
+  apply Empty_eq_spec in HEmp.
+  rewrite fold_init; eauto.
+  - apply fold_identity.
+  - repeat red; intros; subst; now rewrite H1.
+Qed.
+
+Lemma extend_Empty_right_spec (rs rs' : t) :
+  Empty rs' -> eq (extend rs rs') rs.
+Proof. intro HEmp; unfold extend; now rewrite fold_Empty; eauto. Qed.
+
+Lemma extend_add_right_spec (r : resource) (v : Λ) (rs rs' : t) :
+  ~ (In r rs') -> eq (extend rs (add r v rs')) (add r v (extend rs rs')).
+Proof.
+  intro HnIn; unfold extend; rewrite fold_Add; eauto.
+  - reflexivity.
+  - intros k' k Heqk d' d Heqd c c' Heqc; subst; now rewrite Heqc.
+  - apply diamond_add.
+  - unfold SREnvironment.Add; reflexivity.
+Qed.
+
+Lemma valid_extend_spec (k : lvl) (rs rs' : t) :
+  valid k rs -> valid k rs' -> valid k (extend rs rs').
+Proof.
+  revert rs; induction rs' using map_induction; intros rs Hvrs Hvrs'.
+  - rewrite extend_Empty_right_spec; auto.
+  - unfold SREnvironment.Add in H0; rewrite H0 in *; clear H0.
+    rewrite extend_add_right_spec; auto.
+    apply valid_add_notin_spec in Hvrs' as [Hvx [Hve Hvrs'1]]; auto.
+    apply valid_add_spec; auto.
+Qed.
+
+(** **** [new_key] property *)
+
+Lemma new_key_max_spec (x: lvl) (v : Λ) (t : t) :
+  ~ In x t -> new_key (add x v t) = max (new_key t) (S x).
+Proof.
+  intro HnIn.
+  destruct (Nat.leb_spec0 (new_key t) (S x)) as [Hle | Hgt].
+  - rewrite new_key_add_ge_spec; auto; lia.
+  - rewrite new_key_add_lt_spec; auto; lia.
+Qed.
+
+(** **** [init_readers] property *)
+
+#[export] Instance init_func_proper :
+ Proper (Logic.eq ==> Logic.eq ==> RE.eq ==> RE.eq) init_func.
+Proof.
+  intros k' k Heqk d' d Heqd V V' HeqV; subst; unfold init_func.
+  now rewrite HeqV.
+Qed.
+
+Lemma init_func_diamond : Diamond RE.eq init_func.
+Proof.
+  unfold init_func; intros k k' d d' rs rs1 rs' Hneq Heq Heq'.
+  rewrite <- Heq; rewrite <- Heq'.
+  now rewrite RE.add_add_2; auto.
+Qed.
+
+#[local] Hint Resolve init_func_proper init_func_diamond RE.Equal_equiv : core.
+
+Lemma init_readers_Empty_spec (rs : t) (V : 𝐕) :
+  Empty rs -> RE.eq (init_readers rs V) V.
+Proof.
+  intro Hemp; unfold init_readers.
+  rewrite fold_Empty with (eqA := RE.eq); now auto.
+Qed.
+
+Lemma init_readers_add_spec (r : resource) (v : Λ) (rs : t) (V : 𝐕) :
+  ~ (In r rs) ->
+  RE.eq (init_readers (add r v rs) V) (⌈ r ⤆ (⩽ v … ⩾)⌉ (init_readers rs V))%re. 
+Proof.
+  unfold init_readers; intro HnIn.
+  rewrite fold_Add with (eqA := RE.eq); eauto.
+  - unfold init_func at 1; reflexivity.
+  - red; reflexivity.
+Qed.
+
+#[export] Instance init_readers_proper : Proper (eq ==> RE.eq ==> RE.eq) init_readers.
+Proof.
+  intros rs rs' Heqrs V V' HeqV; unfold init_readers.
+  eapply fold_Proper with (eqA := RE.eq); now eauto.
+Qed.
+
+Lemma init_readers_find_spec_1 (rs : t) (V : 𝐕) (r : resource) (v : 𝑣) :
+  ((init_readers rs V)⌊r⌋)%re = Some v -> 
+  find r rs = Some (Cell.extract v) \/ V⌊r⌋%re = Some v.
+Proof.
+  revert r v; induction rs using map_induction; intros r v Hfi.
+  - rewrite init_readers_Empty_spec in Hfi; auto.
+  - unfold SREnvironment.Add in H0; rewrite H0 in *; clear H0.
+    rewrite init_readers_add_spec in Hfi; auto.
+    rewrite RE.add_o in Hfi; destruct (Resource.eq_dec x r) as [| Hneq]; subst.
+    -- inversion Hfi; subst; clear Hfi.
+       left; rewrite add_eq_o; auto.
+    -- apply IHrs1 in Hfi as [Hfi | Hfi]; auto.
+       left; now rewrite add_neq_o.
+Qed. 
+
+Lemma init_readers_find_spec (rs : t) (V : 𝐕) (r : resource) (v : 𝑣) :
+  ((init_readers rs V)⌊r⌋)%re = Some v -> In r rs \/ V⌊r⌋%re = Some v.
+Proof.
+  revert r v; induction rs using map_induction; intros r v Hfi.
+  - rewrite init_readers_Empty_spec in Hfi; auto.
+  - unfold SREnvironment.Add in H0; rewrite H0 in *; clear H0.
+    rewrite init_readers_add_spec in Hfi; auto.
+    rewrite RE.add_o in Hfi; destruct (Resource.eq_dec x r) as [| Hneq]; subst.
+    -- now rewrite add_in_iff; repeat left.
+    -- rewrite add_in_iff.
+       apply IHrs1 in Hfi as [HIn | Hfi]; auto.
+Qed.
+
+
+Lemma init_readers_find_inp_spec (rs : t) (V : 𝐕) (r : resource) (v : 𝑣) :
+  (forall r, V⌊r⌋%re = Some v -> exists v', v = Cell.inp v') ->
+  ((init_readers rs V)⌊r⌋)%re = Some v -> exists v', v = Cell.inp v'. 
+Proof.
+  revert r v; induction rs using map_induction; intros r v HV Hfi.
+  - rewrite init_readers_Empty_spec in Hfi; auto.
+    now apply (HV r).
+  - unfold SREnvironment.Add in H0; rewrite H0 in *; clear H0.
+    rewrite init_readers_add_spec in Hfi; auto.
+    rewrite RE.add_o in Hfi; destruct (Resource.eq_dec x r) as [| Hneq]; subst.
+    -- inversion Hfi; subst; now exists e.
+    -- apply IHrs1 in Hfi; auto.
+Qed.
+
+Lemma init_readers_in_iff  (rs : t) (V : 𝐕) (r : resource) :
+  (r ∈ (init_readers rs V))%re <-> In r rs \/ (r ∈ V)%re.
+Proof.
+  revert r; induction rs using map_induction; intro r; split.
+  - rewrite init_readers_Empty_spec; auto.
+  - intros [HIn | HIn].
+    -- destruct HIn as [v HM].
+       exfalso; now apply (H r v).
+    -- rewrite init_readers_Empty_spec; auto.
+  - intro HIn.
+    unfold SREnvironment.Add in H0; rewrite H0 in *; clear H0.
+    rewrite init_readers_add_spec in HIn; auto.
+    rewrite add_in_iff.
+    apply RE.add_in_iff in HIn as [| HIn]; subst; auto.
+    apply IHrs1 in HIn as [HIn | HIn]; auto.
+  - unfold SREnvironment.Add in H0; rewrite H0 in *; clear H0.
+    rewrite add_in_iff.
+    rewrite init_readers_add_spec; auto.
+    rewrite RE.add_in_iff.
+    intros [[Heq | HIn] | HIn]; subst; auto; 
+    right; rewrite IHrs1; auto.
+Qed.
+
+
+Lemma init_readers_in_unused (rs : t) (V : 𝐕) (r : resource) :
+  In r rs -> REnvironment.unused r (init_readers rs V).
+Proof.
+  revert r; induction rs using map_induction; intros r HIn.
+  - exfalso; destruct HIn as [v HM]; now apply (H r v).
+  - unfold SREnvironment.Add in H0; rewrite H0 in *; clear H0.
+    rewrite init_readers_add_spec; auto; 
+    apply add_in_iff in HIn as [| HIn]; subst.
+    -- apply RE.unused_add_eq_spec; now red.
+    -- assert (Hneq : r <> x) by (intro; subst; contradiction).
+       apply RE.unused_add_neq_spec; auto.
+Qed.
+
+Lemma init_readers_unused (r : resource) (V : 𝐕) (rs : t) :
+  RE.unused r V -> RE.unused r (init_readers rs V).
+Proof.
+  revert r; induction rs using map_induction; intros r Hunsd.
+  - rewrite init_readers_Empty_spec; auto.
+  - unfold SREnvironment.Add in *; rewrite H0 in *; clear H0.
+    rewrite init_readers_add_spec; auto.
+    destruct (Resource.eq_dec r x) as [| Hneq]; subst.
+    -- apply RE.unused_add_eq_spec; now red.
+    -- apply RE.unused_add_neq_spec; auto.
+Qed.
+
+Lemma init_readers_add_remove (r : resource) (v : Λ) (rs : t) (V : 𝐕) :
+  RE.eq (init_readers (add r v rs) V) (init_readers (add r v rs) (RE.Raw.remove r V)).
+Proof.
+  revert r v V; induction rs using map_induction; intros r v V.
+  - rewrite init_readers_add_spec.
+    -- rewrite init_readers_add_spec.
+       + do 2 (rewrite init_readers_Empty_spec; auto).
+         clear H rs; revert r v; induction V using RE.map_induction; intros r v.
+         ++ assert (RE.eq (RE.Raw.remove r V) V).
+            { 
+              unfold RE.eq; rewrite RE.remove_id.
+              intros [v1 HM]; now apply (H r v1).
+            }
+            now rewrite H0.
+         ++ unfold RE.Add in H0; rewrite H0 in *; clear H0.
+            destruct (Resource.eq_dec r x) as [| Hneq]; subst.
+            * rewrite RE.add_shadow.
+              rewrite RE.add_remove_1.
+              now rewrite RE.add_shadow.
+            * rewrite RE.add_add_2; auto.
+              rewrite RE.remove_add_2; auto.
+              symmetry.
+              rewrite RE.add_add_2; auto.
+              now rewrite IHV1.
+       + intros [v1 HM]; now apply (H r v1).
+    -- intros [v1 HM]; now apply (H r v1).
+  - unfold SREnvironment.Add in *; rewrite H0 in *; clear H0.
+    destruct (Resource.eq_dec r x) as [| Hneq]; subst.
+    -- rewrite add_shadow.
+       now apply IHrs1.
+    -- rewrite add_add_2; auto.
+       rewrite init_readers_add_spec.
+       + symmetry; rewrite init_readers_add_spec.
+         ++ now rewrite <- IHrs1.
+         ++ rewrite add_in_iff; intros [|]; subst; contradiction.
+       + rewrite add_in_iff; intros [|]; subst; contradiction.
+Qed.
+
+Lemma init_readers_add_spec_1 (r : resource) (v : 𝑣) (rs : t) (V : 𝐕) :
+  ~ (In r rs) ->
+  RE.eq (init_readers rs (⌈r ⤆ v⌉ V))%re (⌈r ⤆ v⌉ (init_readers rs V))%re. 
+Proof.
+  revert r v V; induction rs using map_induction; intros r v V HnIn.
+  - now do 2 (rewrite init_readers_Empty_spec; auto).
+  - unfold SREnvironment.Add in H0; rewrite H0 in *; clear H0.
+    assert (r <> x /\ ~In r rs1).
+    { 
+      split; intro; subst.
+      - apply HnIn.
+        rewrite add_in_iff; auto.
+      - apply HnIn.
+        rewrite add_in_iff; auto.
+    }
+    destruct H0 as [Hneq HnIn'].
+    do 2 (rewrite init_readers_add_spec; auto).
+    rewrite RE.add_add_2; auto.
+    now rewrite IHrs1; auto.
+Qed.
+
+
+Lemma init_readers_new_key (V : 𝐕) (t : t) : ((init_readers t V)⁺)%re = max (new_key t) (V⁺)%re.
+Proof.
+  revert V.
+  induction t using map_induction; intro V.
+  - rewrite new_key_Empty_spec; auto; simpl.
+    rewrite init_readers_Empty_spec; auto.
+  - unfold SREnvironment.Add in *; rewrite H0 in *; clear H0.
+    rewrite init_readers_add_remove.
+    rewrite init_readers_add_spec; auto.
+    rewrite new_key_max_spec; auto.
+    rewrite RE.new_key_max_spec.
+    + rewrite IHt1.
+      destruct (RE.In_dec V x).
+      ++ apply RE.new_key_in_remove_spec_1 in i as HI.
+         rewrite HI; lia.
+      ++ apply RE.remove_id in n.
+         rewrite n; lia.
+    + rewrite init_readers_in_iff; intros [|]; auto.
+      rewrite RE.remove_in_iff in H0.
+      destruct H0; auto.
+Qed.
+
+(** **** [init_globals] property *)
+
+Lemma init_globals_Empty_spec (t : t) :
+  Empty t -> RE.eq (init_globals t) (∅)%re.
+Proof. apply init_readers_Empty_spec. Qed.
+
+Lemma init_globals_add_spec (r : resource) (v : Λ) (t : t) :
+  ~ (In r t) ->
+  RE.eq (init_globals (add r v t)) (⌈ r ⤆ (⩽ v … ⩾)⌉ (init_globals t))%re. 
+Proof. apply init_readers_add_spec. Qed.
+
+#[export] Instance init_globals_proper : Proper (eq ==> RE.eq) init_globals.
+Proof. unfold init_globals; intros t t' Heqt; now rewrite Heqt. Qed.  
+
+Lemma init_globals_find_spec (t : t) (r : resource) (v : 𝑣) :
+  ((init_globals t)⌊r⌋)%re = Some v -> In r t.
+Proof. 
+  intros Hfi. 
+  apply init_readers_find_spec in Hfi as [HIn | Hfi]; auto.
+  inversion Hfi.
+Qed.
+
+Lemma init_globals_in_iff  (t : t) (r : resource) :
+  (r ∈ (init_globals t))%re <-> In r t.
+Proof.
+  split; intros HIn. 
+  - apply init_readers_in_iff in HIn as [HIn | HIn]; auto.
+    inversion HIn; inversion H.
+  - now apply init_readers_in_iff; left.
+Qed. 
+
+Lemma init_globals_find_iff (t : t) (v : Λ) (r : resource) : 
+  ((init_globals t)⌊r⌋)%re = Some (⩽v …⩾) <-> find r t = Some v.
+Proof.
+  revert r v; induction t using map_induction; intros r v; split; intro Hfi.
+  - rewrite init_globals_Empty_spec in Hfi; auto. 
+    inversion Hfi.
+  - apply Empty_eq_spec in H.
+    rewrite H in Hfi.
+    inversion Hfi.
+  - unfold SREnvironment.Add in *; rewrite H0 in *; clear H0.
+    rewrite init_globals_add_spec in Hfi; auto.
+    destruct (Resource.eq_dec x r) as [| Hneq]; subst.
+    -- rewrite RE.add_eq_o in Hfi; auto.
+       inversion Hfi; subst; clear Hfi.
+       now rewrite add_eq_o.
+    -- rewrite RE.add_neq_o in Hfi; auto.
+       rewrite add_neq_o; auto.
+       now rewrite <- IHt1.
+  - unfold SREnvironment.Add in *; rewrite H0 in *; clear H0.
+    rewrite init_globals_add_spec; auto.
+    destruct (Resource.eq_dec x r) as [| Hneq]; subst.
+    -- rewrite add_eq_o in Hfi; auto.
+       inversion Hfi; subst; clear Hfi.
+       now rewrite RE.add_eq_o.
+    -- rewrite add_neq_o in Hfi; auto.
+       rewrite RE.add_neq_o; auto.
+       now rewrite IHt1.
+Qed.
+
+Lemma init_globals_in_unused (t : t) (r : resource) :
+  In r t -> RE.unused r (init_globals t).
+Proof. apply init_readers_in_unused. Qed.
+
+Lemma init_globals_find_e_spec (t : t) (v : 𝑣) (r : resource) : 
+  ((init_globals t)⌊r⌋)%re = Some v -> exists v', (v = ⩽ v' … ⩾)%type.
+Proof.
+  revert r v; induction t using map_induction; intros r v Hfi.
+  - rewrite init_globals_Empty_spec in Hfi; auto.
+    inversion Hfi.
+  - unfold SREnvironment.Add in *; rewrite H0 in *; clear H0.
+    rewrite init_globals_add_spec in Hfi; auto.
+    destruct (Resource.eq_dec x r) as [| Hneq]; subst.
+    -- rewrite RE.add_eq_o in Hfi; auto.
+       inversion Hfi; subst; clear Hfi.
+       now exists e.
+    -- rewrite RE.add_neq_o in Hfi; auto.
+       now apply (IHt1 r v).
+Qed.
+
+Lemma init_globals_valid (k : lvl) (t : t) :
+  valid k t <-> (k ⊩ init_globals t)%re.
+Proof.
+  induction t using map_induction; split; intro Hvt.
+  - rewrite init_globals_Empty_spec; auto.
+    apply RE.valid_empty_spec.
+  - now apply valid_Empty_spec.
+  - unfold SREnvironment.Add in H0; rewrite H0 in *; clear H0.
+    apply valid_add_notin_spec in Hvt as [Hvx [Hve Hvt]]; auto.
+    rewrite init_globals_add_spec; auto.
+    apply RE.valid_add_notin_spec.
+    -- now rewrite init_globals_in_iff.
+    -- repeat split; auto.
+       now rewrite <- IHt1.
+  - unfold SREnvironment.Add in H0; rewrite H0 in *; clear H0.
+    rewrite init_globals_add_spec in Hvt; auto.
+    apply RE.valid_add_notin_spec in Hvt as [Hvx [Hve Hvt]]; auto.
+    -- apply valid_add_notin_spec; auto.
+       repeat split; auto.
+       now rewrite IHt1.
+    -- now rewrite init_globals_in_iff.
+Qed.
+
+Lemma init_globals_shift (m n : lvl) (t : t) :
+  RE.eq (init_globals (shift m n t)) ([⧐ m – n] (init_globals t))%re.
+Proof.
+  induction t using map_induction.
+  - rewrite shift_Empty_spec; auto.
+    rewrite init_globals_Empty_spec; auto.
+    rewrite RE.shift_Empty_spec; try reflexivity.
+    apply RE.empty_1.
+  - unfold SREnvironment.Add in *; rewrite H0; clear H0.
+    rewrite shift_add_spec.
+    rewrite init_globals_add_spec.
+    -- rewrite init_globals_add_spec; auto.
+       rewrite RE.shift_add_spec; simpl.
+       now rewrite IHt1.
+    -- now rewrite <- shift_in_iff.
+Qed.
+
+Lemma init_globals_new_key (t : t) : ((init_globals t)⁺)%re = new_key t.
+Proof.
+  induction t using map_induction.
+  - rewrite new_key_Empty_spec; auto.
+    rewrite init_globals_Empty_spec; auto.
+  - unfold SREnvironment.Add in *; rewrite H0 in *; clear H0.
+    rewrite init_globals_add_spec; auto.
+    apply new_key_add_spec with (v := e) in H as H1.
+    destruct H1 as [[Heq Hle] | [Heq Hgt]].
+    -- rewrite Heq.
+       rewrite RE.Ext.new_key_add_ge_spec; auto. 
+       + now rewrite init_globals_in_iff.
+       + now rewrite IHt1.
+    -- rewrite Heq.
+       rewrite RE.Ext.new_key_add_lt_spec; auto. 
+       + now rewrite init_globals_in_iff.
+       + now rewrite IHt1.
+Qed.
+
+(** **** [update_readers] property *)
+
+#[export] Instance update_readers_func_proper :
+ Proper (RE.eq ==> Logic.eq ==> Logic.eq ==> eq ==> eq) update_readers_func.
+Proof.
+  intros V V' HeqV k' k Heqk d' d Heqd rs rs' Heqrs; subst. 
+  unfold update_readers_func; rewrite HeqV.
+  destruct (V' ⌊k⌋)%re; try now rewrite Heqrs.
+  destruct r; now rewrite Heqrs.
+Qed.
+
+#[export] Instance update_readers_func_1_proper (V : 𝐕) :
+ Proper (Logic.eq ==> Logic.eq ==> eq ==> eq) (update_readers_func V).
+Proof. intros k' k Heqk d' d Heqd rs rs' Heqrs; subst; now rewrite Heqrs. Qed.
+
+Lemma update_readers_func_diamond (V : 𝐕) : Diamond eq (update_readers_func V).
+Proof.
+  unfold update_readers_func; intros k k' d d' rs rs1 rs' Hneq Heq Heq'.
+  destruct (V ⌊k⌋)%re; destruct (V ⌊k'⌋)%re; 
+  try (destruct r); try (destruct r0); 
+  rewrite <- Heq; rewrite <- Heq';
+  now rewrite add_add_2; auto.
+Qed.
+
+#[local] Hint Resolve update_readers_func_1_proper update_readers_func_proper 
+                      update_readers_func_diamond RE.Equal_equiv : core.
+
+Lemma update_readers_Empty_spec (rs : t) (V : 𝐕) :
+  Empty rs -> Empty (update_readers rs V).
+Proof.
+  intro Hemp; unfold update_readers.
+  rewrite fold_Empty with (eqA := eq); now auto.
+Qed.
+
+Lemma update_readers_Empty_iff (rs : t) (V : 𝐕) :
+  Empty rs -> eq (update_readers rs V) empty.
+Proof.
+  intro Hemp; unfold update_readers.
+  rewrite fold_Empty with (eqA := eq); now auto.
+Qed.
+
+Lemma update_readers_empty_spec (V : 𝐕) :
+  eq (update_readers empty V) empty.
+Proof.
+  unfold update_readers.
+  rewrite fold_Empty with (eqA := eq); now auto.
+Qed.
+
+Lemma update_readers_Add_some_inp_spec (r : resource) (v v' : Λ) (rs rs' : t) (V : 𝐕) :
+  ~ (In r rs) -> SREnvironment.Add r v rs rs' -> (V⌊r⌋)%re = Some (Cell.inp v') ->
+  eq (update_readers rs' V) (add r v (update_readers rs V)). 
+Proof.
+  unfold update_readers; intros HnIn HA Hfi.
+  rewrite fold_Add with (eqA := eq); eauto.
+  unfold update_readers_func at 1. 
+  now rewrite Hfi.
+Qed.
+
+Lemma update_readers_Add_some_out_spec (r : resource) (v v' : Λ) (rs rs' : t) (V : 𝐕) :
+  ~ (In r rs) -> SREnvironment.Add r v rs rs' -> (V⌊r⌋)%re = Some (Cell.out v') ->
+  eq (update_readers rs' V) (add r v' (update_readers rs V)). 
+Proof.
+  unfold update_readers; intros HnIn HA Hfi.
+  rewrite fold_Add with (eqA := eq); eauto.
+  unfold update_readers_func at 1. 
+  now rewrite Hfi.
+Qed.
+
+Lemma update_readers_Add_none_spec (r : resource) (v : Λ) (rs rs' : t) (V : 𝐕) :
+  ~ (In r rs) -> SREnvironment.Add r v rs rs' -> (V⌊r⌋)%re = None ->
+  eq (update_readers rs' V) (add r v (update_readers rs V)). 
+Proof.
+  unfold update_readers; intros HnIn HA Hfi.
+  rewrite fold_Add with (eqA := eq); eauto.
+  unfold update_readers_func at 1.
+  now rewrite Hfi.
+Qed.
+
+Lemma update_readers_add_some_inp_spec (r : resource) (v v' : Λ) (rs : t) (V : 𝐕) :
+  ~ (In r rs) -> (V⌊r⌋)%re = Some (Cell.inp v') ->
+  eq (update_readers (add r v rs) V) (add r v (update_readers rs V)). 
+Proof.
+  unfold update_readers; intros HnIn Hfi.
+  rewrite fold_Add with (eqA := eq); eauto.
+  - unfold update_readers_func at 1. 
+    now rewrite Hfi.
+  - red; reflexivity.
+Qed.
+
+Lemma update_readers_add_some_out_spec (r : resource) (v v' : Λ) (rs : t) (V : 𝐕) :
+  ~ (In r rs) -> (V⌊r⌋)%re = Some (Cell.out v') ->
+  eq (update_readers (add r v rs) V) (add r v' (update_readers rs V)). 
+Proof.
+  unfold update_readers; intros HnIn Hfi.
+  rewrite fold_Add with (eqA := eq); eauto.
+  - unfold update_readers_func at 1. 
+    now rewrite Hfi.
+  - red; reflexivity.
+Qed.
+
+Lemma update_readers_add_none_spec (r : resource) (v : Λ) (rs : t) (V : 𝐕) :
+  ~ (In r rs) -> (V⌊r⌋)%re = None ->
+  eq (update_readers (add r v rs) V) (add r v (update_readers rs V)). 
+Proof.
+  unfold update_readers; intros HnIn Hfi.
+  rewrite fold_Add with (eqA := eq); eauto.
+  - unfold update_readers_func at 1.
+    now rewrite Hfi.
+  - red; reflexivity.
+Qed.
+
+#[export] Instance update_readers_proper : Proper (eq ==> RE.eq ==> eq) update_readers.
+Proof.
+  intros rs rs' Heqrs V V' HeqV; revert rs' Heqrs V V' HeqV. 
+  induction rs using map_induction; intros rs' Heqrs V V' HeqV.
+  - rewrite update_readers_Empty_iff; auto.
+    rewrite Heqrs in H.
+    rewrite update_readers_Empty_iff; now auto.
+  - destruct ((V⌊x⌋)%re) eqn:Hfi.
+    -- destruct r. 
+       + rewrite (update_readers_Add_some_inp_spec x e λ rs1 rs2); auto.
+         symmetry.
+         rewrite (update_readers_Add_some_inp_spec x e λ rs1 rs'); auto.
+         ++ rewrite <- IHrs1 with (V := V) (V' := V'); now auto.
+         ++ unfold SREnvironment.Add in *; now rewrite <- Heqrs.
+         ++ now rewrite <- HeqV.
+       + rewrite (update_readers_Add_some_out_spec x e λ rs1 rs2); auto.
+         symmetry.
+         rewrite (update_readers_Add_some_out_spec x e λ rs1 rs'); auto.
+         ++ rewrite <- IHrs1 with (V := V) (V' := V'); now auto.
+         ++ unfold SREnvironment.Add in *; now rewrite <- Heqrs.
+         ++ now rewrite <- HeqV.
+    -- rewrite (update_readers_Add_none_spec x e rs1 rs2); auto.
+       symmetry.
+       rewrite (update_readers_Add_none_spec x e rs1 rs'); auto.
+       + rewrite <- IHrs1 with (V := V) (V' := V'); now auto.
+       + unfold SREnvironment.Add in *; now rewrite <- Heqrs.
+       + now rewrite <- HeqV.
+Qed.
+
+Lemma update_readers_in_iff  (rs : t) (V : 𝐕) (r : resource) :
+  In r (update_readers rs V) <-> In r rs.
+Proof.
+  revert r; induction rs using map_induction; intro r; split.
+  - rewrite update_readers_Empty_iff; auto; intro HIn.
+    inversion HIn; inversion H0.
+  - intro HIn.
+    destruct HIn as [v HM].
+    exfalso; now apply (H r v).
+  - intro HIn.
+    unfold SREnvironment.Add in H0; rewrite H0 in *; clear H0.
+    rewrite add_in_iff.
+    destruct ((V⌊x⌋)%re) eqn:Hfi.
+    -- destruct r0.
+       + rewrite update_readers_add_some_inp_spec with (v' := λ) in HIn; auto.
+         apply add_in_iff in HIn as [Heq | HIn]; auto.
+         right; now rewrite <- IHrs1.
+       + rewrite update_readers_add_some_out_spec with (v' := λ) in HIn; auto.
+         apply add_in_iff in HIn as [Heq | HIn]; auto.
+         right; now rewrite <- IHrs1.
+    -- rewrite update_readers_add_none_spec in HIn; auto.
+       apply add_in_iff in HIn as [Heq | HIn]; auto.
+       right; now rewrite <- IHrs1.
+  - intro HIn.
+    unfold SREnvironment.Add in H0; rewrite H0 in *; clear H0.
+    destruct ((V⌊x⌋)%re) eqn:Hfi.
+    -- destruct r0.
+       + rewrite update_readers_add_some_inp_spec with (v' := λ); auto.
+         rewrite add_in_iff.
+         apply add_in_iff in HIn as [Heq | HIn]; auto.
+         right; now rewrite IHrs1.
+       + rewrite update_readers_add_some_out_spec with (v' := λ); auto.
+         rewrite add_in_iff.
+         apply add_in_iff in HIn as [Heq | HIn]; auto.
+         right; now rewrite IHrs1.
+    -- rewrite update_readers_add_none_spec; auto.
+       rewrite add_in_iff.
+       apply add_in_iff in HIn as [Heq | HIn]; auto.
+       right; now rewrite IHrs1.
+Qed.
+
+(** **** [halts] property *)
+
+Lemma halts_union_spec (k : lvl) (rs rs': t) :
+  halts k rs /\ halts k rs' -> halts k (extend rs rs').
+Proof.
+  unfold halts; intros [HFa HFa'] r v Hfi.
+  apply find_2 in Hfi. 
+  apply extend_mapsto_iff in Hfi as [HM | [HM _]]; apply find_1 in HM.
+  - now apply (HFa' r).
+  - now apply (HFa r).
+Qed.
+
+Lemma halts_add_spec (k : lvl) (r : resource) (v : Λ) (rs : t) :
+  (ET.halts k v) /\ halts k rs -> halts k (add r v rs).
+Proof.
+  intros [Hltv Hlts] r' v' Hfi.
+  rewrite add_o in Hfi; destruct (Resource.eq_dec r r') as [| Hneq]; subst.
+  - inversion Hfi; subst; auto.
+  - apply Hlts in Hfi; auto.
+Qed.
+
+Lemma halts_add_iff (k : lvl) (r : resource) (v : Λ) (rs : t) :
+  ~ (In r rs) -> 
+  halts k (add r v rs) <-> (ET.halts k v) /\ halts k rs.
+Proof.
+  intros HIn; split.
+  - unfold halts; intro HFa.
+    apply For_all_add_notin_spec in HFa; auto.
+  - apply halts_add_spec.
+Qed.
+
+Lemma halts_weakening (m n : lvl) (rs : t) : 
+  m <= n -> halts m rs -> halts n (shift m (n - m) rs).
+Proof.
+  intros Hle Hlt r v Hfi. 
+  apply shift_find_e_spec_1 in Hfi as HI.
+  destruct HI as [[r' Heqr'] [v' Heqv']]; subst.
+  rewrite <- shift_find_iff in Hfi. 
+  apply ET.halts_weakening; auto; apply Hlt in Hfi; now simpl in *.
+Qed.
+
+Lemma halts_weakening_1 (m n : lvl) (rs : t) : 
+  halts m rs -> halts (m + n) (shift m n rs).
+Proof.
+  intro Hlt; replace n with ((m + n) - m) at 2 by lia.
+  apply halts_weakening; auto; lia.
+Qed.
+
+Lemma halts_init_readers (k : lvl) (rs : t) (V : 𝐕) :
+  halts k rs -> RE.halts k V -> RE.halts k (init_readers rs V).
+Proof.
+  induction rs using map_induction; intros Hltrs HltV.
+  - now rewrite init_readers_Empty_spec.
+  - unfold SREnvironment.Add in H0; rewrite H0 in *; clear H0.
+    rewrite init_readers_add_spec; auto.
+    apply RE.halts_add_spec; simpl.
+    apply halts_add_iff in Hltrs as [Hkte Htlrs1]; auto. 
+Qed.
+
+Lemma halts_init_globals (k : lvl) (rs : t) :
+  halts k rs -> RE.halts k (init_globals rs).
+Proof.
+  intro Hlt; apply halts_init_readers; auto.
+  intros r d Hfi; inversion Hfi.
+Qed.
+
+Lemma halts_update_readers (k : lvl) (rs : t) (V : 𝐕) :
+  halts k rs -> RE.halts k V -> halts k (update_readers rs V).
+Proof.
+  induction rs using map_induction; intros Hltrs HltV.
+  - now rewrite update_readers_Empty_iff.
+  - unfold SREnvironment.Add in H0; rewrite H0 in *; clear H0.
+    destruct ((V⌊x⌋)%re) eqn:Hfi.
+    -- destruct r.
+       + rewrite update_readers_add_some_inp_spec; eauto.
+         rewrite halts_add_iff in *; auto.
+         ++ destruct Hltrs; split; auto.
+         ++ now rewrite update_readers_in_iff.
+       + rewrite update_readers_add_some_out_spec; eauto.
+         rewrite halts_add_iff in *; auto.
+         ++ destruct Hltrs; split; auto.
+            apply HltV in Hfi; now simpl in *.
+         ++ now rewrite update_readers_in_iff.
+    -- rewrite update_readers_add_none_spec; eauto.
+       rewrite halts_add_iff in *; auto.
+       ++ destruct Hltrs; split; auto.
+       ++ now rewrite update_readers_in_iff.
+Qed.
+
+(** **** Morphism *)
+
+#[export] Instance in_SREnvironment : Proper (Logic.eq ==> eq ==> iff) In.
+Proof. intros k' k Heqk rs rs' Heqrs; subst; now rewrite Heqrs. Qed.
+
+#[export] Instance Add_SREnvironment : 
+  Proper (Resource.eq ==> Term.eq ==> eq ==> eq ==> iff) (@SREnvironment.Add Term.t).
+Proof.
+  intros k' k Heqk d d' Heqd rs rs' Heqrs rs1 rs1' Heqrs1; unfold SREnvironment.Add.
+  now rewrite Heqk, Heqd, Heqrs, Heqrs1. 
+Qed.
+
+#[export] Instance halts_SREnvironment : Proper (Logic.eq ==> eq ==> iff) halts. 
+Proof. unfold halts; intros m n Heqm rs rs' Heqrs; subst; now rewrite Heqrs. Qed.
+
+End SREnvironment.
+
+(** ---- *)
+
+(** ** Notation - Virtual Resource Environment - Reader *)
+
+Module SREnvironmentNotations.
+
+(** *** Scope *)
+Declare Scope srenv_scope.
+Delimit Scope srenv_scope with sr.
+
+(** *** Notation *)
+Definition 𝐄 := SREnvironment.t.
+
+Notation "t '⁺'" := (SREnvironment.Ext.new_key t) (at level 16) : srenv_scope.
+Notation "∅" := SREnvironment.Raw.empty (at level 0, no associativity) : srenv_scope. 
+Notation "r '∉' t" := (~ (SREnvironment.Raw.In r t)) (at level 75, no associativity) : srenv_scope. 
+Notation "'isEmpty(' t ')'" := (SREnvironment.Empty t) (at level 20, no associativity) : srenv_scope. 
+Notation "'Add'" := (SREnvironment.Add) (at level 20, no associativity) : srenv_scope. 
+Notation "t '⌊' x '⌋'"  := (SREnvironment.Raw.find x t) (at level 15, x constr) : srenv_scope.
+Notation "'max(' t ')'"  := (SREnvironment.Ext.max_key t) (at level 15) : srenv_scope.
+Notation "⌈ x ⤆ v '⌉' t" := (SREnvironment.Raw.add x v t) 
+                             (at level 15, x constr, v constr) : srenv_scope.
+Notation "'[⧐' lb '–' k ']' t" := (SREnvironment.shift lb k t) 
+                                   (at level 65, right associativity) : srenv_scope.
+
+Infix "⊆" := SREnvironment.Submap (at level 60, no associativity) : srenv_scope. 
+Infix "∈" := SREnvironment.Raw.In (at level 60, no associativity) : srenv_scope. 
+Infix "=" := SREnvironment.eq : srenv_scope.
+Infix "∪" := SREnvironment.extend : srenv_scope.
+Infix "⊩" := SREnvironment.valid (at level 20, no associativity) : srenv_scope.
+
+(** *** Morphism *)
+
+Import SREnvironment.
+
+#[export] Instance equiv_sr : Equivalence SREnvironment.eq := _.
+#[export] Instance max_sr : Proper (eq ==> Logic.eq) (Ext.max_key) := Ext.max_key_eq.
+#[export] Instance new_sr : Proper (eq ==> Logic.eq) (Ext.new_key) := Ext.new_key_eq.
+#[export] Instance in_sr : Proper (Logic.eq ==> SREnvironment.eq ==> iff) (SREnvironment.Raw.In) := _.
+#[export] Instance find_sr : Proper (Logic.eq ==> eq ==> Logic.eq) (Raw.find) := _.
+#[export] Instance Empty_sr : Proper (SREnvironment.eq ==> iff) (SREnvironment.Empty) := _.
+#[export] Instance Add_sr : 
+  Proper (Resource.eq ==> Term.eq ==> eq ==> eq ==> iff) (@SREnvironment.Add Term.t) := _.
+#[export] Instance add_sr : 
+  Proper (Resource.eq ==> Term.eq ==> eq ==> eq) (@Raw.add Term.t) := _.
+#[export] Instance Submap_sr : Proper (eq ==> eq ==> iff) Submap := _.
+#[export] Instance Submap_sr_po : PreOrder SREnvironment.Submap := Submap_po.
+#[export] Instance valid_sr : Proper (Logic.eq ==> SREnvironment.eq ==> iff) SREnvironment.valid := _.
+#[export] Instance shift_sr : Proper (Logic.eq ==> Logic.eq ==> eq ==> eq) shift := _.
+#[export] Instance halts_sr: Proper (Logic.eq ==> SREnvironment.eq ==> iff) SREnvironment.halts := _.
+
+End SREnvironmentNotations.
